refocusing_lang.v
@@ -15,7 +15,7 @@ Module Type RED_LANG.
   Coercion ckind_L2any (kL : ckind_L) := proj1_sig kL.*)
 
   Axiom ckind_death_propagation : 
-      forall k, dead_ckind k -> forall ec, dead_ckind (k+>ec). 
+      forall k, dead_ckind k -> forall ec, dead_ckind (k+>ec).
 
 
   Inductive context : ckind -> ckind -> Set :=
@@ -128,20 +128,24 @@ Module Type RED_REF_LANG.
   Parameter dec_term    : term -> forall k, interm_dec k.
   Parameter dec_context : forall ec k, value (k+>ec) -> interm_dec k.
 
+
   Axiom dec_term_liveness : 
       forall {t k t0 ec0}, dec_term t k = in_term t0 ec0 -> ~ dead_ckind (k+>ec0).
+
 
   Inductive subterm_one_step : term -> term -> Prop :=
   | st_1 : forall t t0 ec, t = atom_plug t0 ec -> subterm_one_step t0 t.
   Axiom wf_st1 : well_founded subterm_one_step.
 
+
   Definition subterm_order := clos_trans_1n term subterm_one_step.
   Notation " a <| b " := (subterm_order a b) (at level 40, no associativity).
   Definition wf_sto : well_founded subterm_order := wf_clos_trans_l _ _ wf_st1.
 
-  Parameter ec_order : ckind -> elem_context -> elem_context -> Prop.
-  Notation "k |~  a << b " := (ec_order k a b) (at level 40, no associativity).
-  Axiom wf_eco : forall k, well_founded (ec_order k).
+
+  Parameter ec_order : ckind -> term -> elem_context -> elem_context -> Prop.
+  Notation "k , t |~  ec1 << ec2 " := (ec_order k t ec1 ec2) (at level 40, no associativity).
+  Axiom wf_eco : forall k t, well_founded (ec_order k t).
 
 
   (*Definition ec_proper_sub ec t k := 
@@ -160,20 +164,22 @@ Module Type RED_REF_LANG.
   Axiom dec_term_val_empty  : forall t k v, 
                                   dec_term t k = in_val v -> only_empty t k.
   Axiom dec_term_term_top   : forall t t' k ec, 
-            dec_term t k = in_term t' ec -> forall ec', ~ k |~ ec << ec'.
+            dec_term t k = in_term t' ec -> forall ec', ~ k, t |~ ec << ec'.
   Axiom dec_context_red_bot : 
       forall k ec v r, dec_context ec k v = in_red r -> 
-          forall ec' t', atom_plug t' ec' = atom_plug (value_to_term v) ec -> 
-              ~ k |~ ec' << ec.
-  Axiom dec_context_val_bot : forall k ec v v', 
-            dec_context ec k v = R.in_val v' -> forall ec', ~ k |~ ec' << ec.
+          forall ec', ~ k, (atom_plug v ec) |~ ec' << ec.
+  Axiom dec_context_val_bot : 
+      forall k ec v v', dec_context ec k v = in_val v' -> 
+          forall ec', ~ k, (atom_plug v ec) |~ ec' << ec.
   Axiom dec_context_term_next : 
-      forall ec k v t ec', dec_context ec k v = in_term t ec' -> 
-      k |~ ec' << ec /\ forall ec'', k |~ ec'' << ec -> ~ k |~ ec' << ec''.
-  Axiom dec_term_ec_most_transitable : forall {t0 ec0 t1 ec1 k},
+      forall ec0 k v t ec1, dec_context ec0 k v = in_term t ec1 -> 
+          k, (atom_plug v ec0) |~ ec1 << ec0 /\ 
+          forall ec,    k, (atom_plug v ec0) |~ ec  << ec0  ->  
+                      ~ k, (atom_plug v ec0) |~ ec1 << ec.
+  (*Axiom dec_term_ec_most_transitable : forall {t0 ec0 t1 ec1 k},
       transitable_from k ec1 ->
       dec_term (atom_plug t1 ec1) k = in_term t0 ec0 ->
-      transitable_from k ec0.
+      transitable_from k ec0.*)
 
   Axiom dec_term_correct : forall t k, match dec_term t k with
       | in_red r      => redex_to_term r = t
@@ -181,57 +187,41 @@ Module Type RED_REF_LANG.
       | in_term t' ec => atom_plug t' ec = t
       | in_dead       => dead_ckind k 
       end.
+
   Axiom dec_context_correct : forall ec k v, match dec_context ec k v with
       | in_red r      => redex_to_term r = atom_plug v ec
       | in_val v'     => value_to_term v' = atom_plug v ec
       | in_term t ec' => atom_plug t ec' = atom_plug v ec
       | in_dead       => dead_ckind (k+>ec) 
       end.
+
   Axiom dec_term_from_dead : 
       forall t k, dead_ckind k -> dec_term t k = in_dead k.
+
   Axiom dec_context_from_dead : 
-      forall ec k v, dead_ckind (ckind_trans k ec) -> dec_context ec k v = in_dead k.
+      forall ec k v, dead_ckind (k+>ec) -> dec_context ec k v = in_dead k.
 
+  Definition strict_ec ec t := exists t', atom_plug t' ec = t. 
 
-  Axiom ec_order_antisym : forall k ec ec0, 
-      k |~ ec << ec0 -> ~ k |~ ec0 << ec.
-  Axiom ec_order_trans : forall k ec0 ec1 ec2,
-      k |~ ec0 << ec1 -> k |~ ec1 << ec2 -> k |~ ec0 << ec2.
+  Axiom ec_order_antisym : forall k t ec ec0, 
+      k,t |~ ec << ec0 -> ~ k,t |~ ec0 << ec.
+  Axiom ec_order_trans : forall k t ec0 ec1 ec2,
+      k,t |~ ec0 << ec1 -> k,t |~ ec1 << ec2 -> k,t |~ ec0 << ec2.
   Axiom ec_order_comp_if :
-      forall ec0 ec1, ec_siblings ec0 ec1 -> 
-      forall k, transitable_from k ec0 -> transitable_from k ec1 ->
-      k |~ ec0 << ec1 \/ k |~ ec1 << ec0 \/ ec0 = ec1.
+      forall t ec0 ec1, strict_ec ec0 t -> strict_ec ec1 t -> 
+          forall k, ~ dead_ckind (k+>ec0) -> ~ dead_ckind (k+>ec1) ->
+              k,t |~ ec0 << ec1 \/ k,t |~ ec1 << ec0 \/ ec0 = ec1.
   Axiom ec_order_comp_fi :
-      forall ec0 ec1 k, k |~ ec0 << ec1 ->
-      ec_siblings ec0 ec1 /\ transitable_from k ec0 /\ transitable_from k ec1.
+      forall k t ec0 ec1,  k, t |~ ec0 << ec1 ->
+          strict_ec ec0 t /\ strict_ec ec1 t /\ 
+          ~ dead_ckind (k+>ec0) /\ ~ dead_ckind (k+>ec1).
 
-  Axiom elem_context_det : forall t0 t1 k ec0 ec1,
-      k |~ ec0 << ec1 -> atom_plug t0 ec0 = atom_plug t1 ec1 ->
-      exists v : R.value (k+>ec1), t1 = value_to_term v.
+  Axiom elem_context_det : 
+      forall t k ec0 ec1,  k, t |~ ec0 << ec1 -> 
+          exists (v : value (k+>ec1)), t = atom_plug v ec1.
 
 End RED_REF_LANG.
 
-(*
-Module RED_REF_LANG_Facts (R : RED_REF_LANG) (RP : LANG_PROP R.R).
-
-  Import R.R.
-
-  Lemma indecomp_proper_ec :
-      forall {k1 k2} (c : context k1 k2) ec t, 
-          R.indecomp_proper (ec=:c) t -> R.indecomp_proper c (atom_plug t ec).
-
-  Proof with eauto.
-  unfold R.indecomp_proper.
-  intros.
-  cut (R.ec_proper_sub ec0 (plug t (((ec=:[_]) ~+ c0) ~+ ec0 =: [_])) k).
-  eauto.
-
-  apply H with (c1:=c1); simpl.
-  apply f_equal...
-  Qed.
-
-End RED_REF_LANG_Facts.
-*)
 
   Ltac prove_st_wf := 
       intro a; constructor; induction a; 
@@ -242,11 +232,11 @@ End RED_REF_LANG_Facts.
           constructor; auto
       ).
   Ltac prove_ec_wf := 
-      intros k a; destruct k, a; repeat 
+      intros k t ec; destruct k, t, ec; repeat 
       (
           constructor; 
-          intros ec T; 
-          destruct ec; inversion T; subst; clear T
+          intros ec H; 
+          destruct ec; inversion H; dep_subst; clear H
       ).
 
 
